Let $n = 1010$. The sum is over $0 \le k \le 3^n - 1$.
The function $f(k)$ is the number of ones in the base 3 representation of $k$.
The base 3 representation of $k$ is $(d_{n-1} d_{n-2} \dots d_0)_3$, where $d_i \in \{0, 1, 2\}$.
Then $f(k) = \sum_{i=0}^{n-1} I(d_i = 1)$, and $(-2)^{f(k)} = \prod_{i=0}^{n-1} (-2)^{I(d_i = 1)}$.

Let $P(z) = \sum_{k=0}^{3^n-1} (-2)^{f(k)} (z+k)^{2023}$.
We are looking for the values of $z$ for which $P(z) = 0$.
The degree of the polynomial is 2023.

Consider a simpler case: $n=1$. Then $0 \le k \le 3^1 - 1 = 2$.
$k=0 = (0)_3, f(0) = 0, (-2)^{f(0)} = 1$.
$k=1 = (1)_3, f(1) = 1, (-2)^{f(1)} = -2$.
$k=2 = (2)_3, f(2) = 0, (-2)^{f(2)} = 1$.
The sum is $\sum_{k=0}^{2} (-2)^{f(k)} (z+k)^{2023} = 1 \cdot (z+0)^{2023} + (-2) \cdot (z+1)^{2023} + 1 \cdot (z+2)^{2023} = z^{2023} - 2(z+1)^{2023} + (z+2)^{2023}$.
If this is zero for all $z$, then the coefficients of each power of $z$ must be zero.
The coefficient of $z^{2023}$ is $1 - 2 + 1 = 0$.
The coefficient of $z^{2022}$ is $\binom{2023}{2022} (0^0 - 2 \cdot 1^1 + 1 \cdot 2^1) = 2023 (0 - 2 + 2) = 0$.

Let $y = z + \frac{3^n-1}{2}$. Then $z = y - \frac{3^n-1}{2}$.
When $k$ goes from $0$ to $3^n-1$, $k - \frac{3^n-1}{2}$ goes from $-\frac{3^n-1}{2}$ to $\frac{3^n-1}{2}$.
Let $k' = k - \frac{3^n-1}{2}$. Then $k = k' + \frac{3^n-1}{2}$.
The sum becomes $\sum_{k=0}^{3^n-1} (-2)^{f(k)} (y - \frac{3^n-1}{2} + k)^{2023} = 0$.

Consider the case when $2023 = 1$.
$\sum_{k=0}^{3^n-1} (-2)^{f(k)} (z+k) = z \sum_{k=0}^{3^n-1} (-2)^{f(k)} + \sum_{k=0}^{3^n-1} (-2)^{f(k)} k$.
$\sum_{k=0}^{3^n-1} (-2)^{f(k)} = \sum_{d_0=0}^2 \dots \sum_{d_{n-1}=0}^2 \prod_{i=0}^{n-1} (-2)^{I(d_i=1)} = \prod_{i=0}^{n-1} \sum_{d_i=0}^2 (-2)^{I(d_i=1)} = \prod_{i=0}^{n-1} ((-2)^0 + (-2)^1 + (-2)^0) = \prod_{i=0}^{n-1} (1 - 2 + 1) = 0$.
$\sum_{k=0}^{3^n-1} (-2)^{f(k)} k = \sum_{d_0=0}^2 \dots \sum_{d_{n-1}=0}^2 \left( \prod_{i=0}^{n-1} (-2)^{I(d_i=1)} \right) \sum_{j=0}^{n-1} d_j 3^j$.
$= \sum_{j=0}^{n-1} 3^j \sum_{d_0=0}^2 \dots \sum_{d_{n-1}=0}^2 \left( \prod_{i=0}^{n-1} (-2)^{I(d_i=1)} \right) d_j$.
$= \sum_{j=0}^{n-1} 3^j \left( \prod_{i \ne j} \sum_{d_i=0}^2 (-2)^{I(d_i=1)} \right) \sum_{d_j=0}^2 (-2)^{I(d_j=1)} d_j$.
$= \sum_{j=0}^{n-1} 3^j \cdot 0 \cdot ((-2)^0 \cdot 0 + (-2)^1 \cdot 1 + (-2)^0 \cdot 2) = 0$.
So for degree 1, the equation is $0 = 0$, true for all $z$.

Let $g(x) = (-2)^{f(x)}$.
The sum is $\sum_{k=0}^{3^n-1} g(k) (z+k)^{2023} = 0$.
Consider the transformation $k' = 3^n - 1 - k$.
$f(k') = $ number of ones in base 3 of $3^n - 1 - k$.
$3^n - 1 = (22\dots2)_3$ (n times).
If the digits of $k$ are $d_{n-1} \dots d_0$, the digits of $3^n - 1 - k$ are $2-d_{n-1}, \dots, 2-d_0$.
$f(k') = \sum_{i=0}^{n-1} I(2-d_i = 1) = \sum_{i=0}^{n-1} I(d_i = 1) = f(k)$.
So $g(k') = g(k)$.
When $k$ goes from $0$ to $3^n-1$, $3^n-1-k$ goes from $3^n-1$ to $0$.
Let the sum be $S$.
$S = \sum_{k=0}^{3^n-1} g(k) (z+k)^{2023}$.
Let $j = 3^n - 1 - k$, so $k = 3^n - 1 - j$.
$S = \sum_{j=3^n-1}^{0} g(3^n-1-j) (z + 3^n - 1 - j)^{2023} (-1)$.
$S = \sum_{j=0}^{3^n-1} g(j) (z + 3^n - 1 - j)^{2023}$.
So we have $\sum_{k=0}^{3^n-1} g(k) (z+k)^{2023} = \sum_{k=0}^{3^n-1} g(k) (z + 3^n - 1 - k)^{2023}$.
$\sum_{k=0}^{3^n-1} g(k) [ (z+k)^{2023} - (z + 3^n - 1 - k)^{2023} ] = 0$.

Let $m = \frac{3^n-1}{2}$.
Consider $z = -m = -\frac{3^n-1}{2}$.
Then $z+k = k - m$, $z+3^n-1-k = 3^n-1-k - m = 3^n-1-k - \frac{3^n-1}{2} = \frac{3^n-1}{2} - k = m - k$.
$(z+k)^{2023} = (k-m)^{2023}$.
$(z+3^n-1-k)^{2023} = (m-k)^{2023} = (-1)^{2023} (k-m)^{2023} = -(k-m)^{2023}$.
So $(z+k)^{2023} - (z+3^n-1-k)^{2023} = (k-m)^{2023} - (-(k-m)^{2023}) = 2(k-m)^{2023}$.
The sum becomes $\sum_{k=0}^{3^n-1} g(k) 2(k-m)^{2023} = 0$.

Let $y = z + \frac{3^n-1}{2}$. Then $z = y - \frac{3^n-1}{2}$.
The equation is $\sum_{k=0}^{3^n-1} (-2)^{f(k)} (y - \frac{3^n-1}{2} + k)^{2023} = 0$.
Let $j = k - \frac{3^n-1}{2}$. When $k=0, j = -\frac{3^n-1}{2}$. When $k=3^n-1, j = 3^n-1 - \frac{3^n-1}{2} = \frac{3^n-1}{2}$.
The terms are symmetric around $\frac{3^n-1}{2}$.
Consider the case $n=1$. $m=1$.
$\sum_{k=0}^2 (-2)^{f(k)} (z+k)^{2023} = (z)^2023 - 2(z+1)^{2023} + (z+2)^{2023}$.
If $z=-1$, $(-1)^{2023} - 2(0)^{2023} + (1)^{2023} = -1 - 0 + 1 = 0$.
$-\frac{3^1-1}{2} = -1$.

Consider the polynomial $P(x) = x^{2023}$.
The sum is $\sum_{k=0}^{3^n-1} (-2)^{f(k)} P(z+k) = 0$.
Consider the finite difference operator $\Delta_h f(x) = f(x+h) - f(x)$.
Consider the third order difference: $P(z) - 2 P(z+1) + P(z+2)$.
If $P(x) = x$, $z - 2(z+1) + (z+2) = z - 2z - 2 + z + 2 = 0$.
If $P(x) = x^2$, $z^2 - 2(z+1)^2 + (z+2)^2 = z^2 - 2(z^2+2z+1) + (z^2+4z+4) = z^2 - 2z^2 - 4z - 2 + z^2 + 4z + 4 = 2$.
If $P(x) = x^3$, $z^3 - 2(z+1)^3 + (z+2)^3 = z^3 - 2(z^3+3z^2+3z+1) + (z^3+6z^2+12z+8) = z^3 - 2z^3 - 6z^2 - 6z - 2 + z^3 + 6z^2 + 12z + 8 = 6z + 6$.

Let $E$ be the shift operator, $E f(x) = f(x+1)$.
The operator is $I - 2 E + E^2 = (I-E)^2$.
The sum is $\sum_{k=0}^{3^n-1} \prod_{i=0}^{n-1} (-2)^{I(d_i=1)} (z+k)^{2023}$.
Consider the operator $\prod_{i=0}^{n-1} (I - 2 E^{3^i} + E^{2 \cdot 3^i})$.
This is related to the base 3 representation.

Let $Q(z) = \sum_{k=0}^{3^n-1} (-2)^{f(k)} e^{(z+k)t}$.
$Q(z) = e^{zt} \sum_{k=0}^{3^n-1} (-2)^{f(k)} e^{kt}$.
$k = \sum_{i=0}^{n-1} d_i 3^i$.
$e^{kt} = e^{\sum_{i=0}^{n-1} d_i 3^i t} = \prod_{i=0}^{n-1} e^{d_i 3^i t}$.
$\sum_{k=0}^{3^n-1} (-2)^{f(k)} e^{kt} = \sum_{d_0=0}^2 \dots \sum_{d_{n-1}=0}^2 \prod_{i=0}^{n-1} (-2)^{I(d_i=1)} e^{d_i 3^i t}$.
$= \prod_{i=0}^{n-1} \sum_{d_i=0}^2 (-2)^{I(d_i=1)} e^{d_i 3^i t}$.
$= \prod_{i=0}^{n-1} ( (-2)^0 e^{0 \cdot 3^i t} + (-2)^1 e^{1 \cdot 3^i t} + (-2)^0 e^{2 \cdot 3^i t} )$.
$= \prod_{i=0}^{n-1} ( 1 - 2 e^{3^i t} + e^{2 \cdot 3^i t} ) = \prod_{i=0}^{n-1} (1 - e^{3^i t})^2$.

We need the coefficient of $\frac{t^{2023}}{2023!}$ in $Q(z)$ to be zero.
Coefficient of $t^m$ in $e^{(z+k)t}$ is $\frac{(z+k)^m}{m!}$.
Coefficient of $t^{2023}$ in $Q(z)$ is $\sum_{k=0}^{3^n-1} (-2)^{f(k)} \frac{(z+k)^{2023}}{2023!}$.

The equation is $\sum_{k=0}^{3^n-1} (-2)^{f(k)} (z+k)^{2023} = 0$.
Let $P(x) = x^{2023}$.
The operation is like applying a difference operator.
Consider the operator $\Delta_a f(x) = f(x+a) - f(x)$.
Consider the operator that maps $P(z)$ to $\sum_{k=0}^{3^n-1} (-2)^{f(k)} P(z+k)$.
Let $n=1$. $P(z) - 2 P(z+1) + P(z+2)$.
If $P(z) = c$, $c - 2c + c = 0$.
If $P(z) = z - a$, $(z-a) - 2(z+1-a) + (z+2-a) = z-a - 2z-2+2a + z+2-a = 0$.
If $P(z) = (z-a)^2$, $(z-a)^2 - 2(z+1-a)^2 + (z+2-a)^2 = 2$.

Let $m = \frac{3^n-1}{2}$. Consider the symmetry around $-m$.
Let $z = -m$.
The equation holds.

Consider the roots of $\prod_{i=0}^{n-1} (1 - e^{3^i t})^2 = 0$.
$1 - e^{3^i t} = 0$, $e^{3^i t} = 1$, $3^i t = 2 \pi i k_i$, $t = \frac{2 \pi i k_i}{3^i}$, $k_i \in \mathbb{Z}$.

Let $F(z) = \sum_{k=0}^{3^n-1} (-2)^{f(k)} e^{kt}$.
$F(z) = \prod_{i=0}^{n-1} (1 - e^{3^i t})^2$.
The roots are when $e^{3^i t} = 1$.

Consider the polynomial $Q(z) = \sum_{k=0}^{3^n-1} (-2)^{f(k)} (z+k)^{2023}$.
Degree of $Q(z)$ is 2023.
We found one root $z = -\frac{3^n-1}{2}$.

The given roots are related to the centroid of the indices with weights.
Consider the case when $2023=0$.
$\sum_{k=0}^{3^n-1} (-2)^{f(k)} = 0$.

Consider the case when $2023=1$.
$\sum_{k=0}^{3^n-1} (-2)^{f(k)} (z+k) = z \sum_{k=0}^{3^n-1} (-2)^{f(k)} + \sum_{k=0}^{3^n-1} (-2)^{f(k)} k = 0$.

The problem seems to be related to moments.
Let the measure $\mu$ on $\{0, 1, \dots, 3^n-1\}$ be $\mu(\{k\}) = (-2)^{f(k)}$.
The equation is $\sum_{k=0}^{3^n-1} \mu(\{k\}) (z+k)^{2023} = 0$.
The first moment is $\sum_{k=0}^{3^n-1} (-2)^{f(k)} k = 0$.
The zeroth moment is $\sum_{k=0}^{3^n-1} (-2)^{f(k)} = 0$.

Consider the center of mass with weights $(-2)^{f(k)}$.
The average value is $\frac{\sum_{k=0}^{3^n-1} (-2)^{f(k)} k}{\sum_{k=0}^{3^n-1} (-2)^{f(k)}}$, which is $0/0$.

Let $m = \frac{3^n-1}{2}$.
The roots are related to $-m$.
Consider the second moment.
$\sum_{k=0}^{3^n-1} (-2)^{f(k)} k^2 = \sum_{j=0}^{n-1} \sum_{l=0}^{n-1} 3^{j+l} \sum_{d} (\dots) d_j d_l$.
If $j \ne l$, the sum is 0.
If $j = l$, the sum is $\sum_{j=0}^{n-1} 3^{2j} \sum_{d} (\dots) d_j^2 = \sum_{j=0}^{n-1} 3^{2j} \cdot 0 \cdot (0^2 \cdot 1 + 1^2 \cdot (-2) + 2^2 \cdot 1) = 0$.

The roots are $z_0$ such that the first $2023+1$ moments of the measure around $-z_0$ are zero.
The measure has $3^n$ points.
